
![[Pasted image 20240729115434.png]]

1.

$$
\Sigma^{*} = \{ a, b, c, d, aa, ab, ac, ad, \dots \} = \Sigma^{0} \cup \Sigma^{1} \cup \Sigma^{2}\dots
$$

2.

$$
\begin{align}
BS : u^{0} = \lambda  \\
RS : u^{n} = u \cdot u^{n-1}
\end{align}
$$

3.

$$
\begin{align}
BS : |\lambda| = 0  \\
RS : |u| = |av| = 1 + |v|
\end{align}
$$
4.

$$
\begin{align}
BS: \lambda^{R} = \lambda \\
RS: u^{R} = (va)^{R} = av^{R}
\end{align}
$$

5.


$$
\begin{align}
F(\lambda) &: (u\lambda)^{R}  = \lambda^{R}u^{R} \\
F(\lambda) &: \lambda u^{R}  = \lambda u^{R}  \\
F(\lambda) &: u^{R} = u^{R}
\end{align}
$$

$$
\begin{align}
F(\lambda a) &: (u\lambda a)^{R} = (\lambda a)^{R} u^{R}  \\
&: a (u\lambda)^{R} = a\lambda^{R} u^{R} \\
&: a\lambda u^{R} = a \lambda u^{R}
\end{align}
$$

$$
\begin{align}
F((uva)^{R}) &: a (uv)^{R} \\
 &: a u^{R}v^{R} \\
 &: (ua)^{R} v^{R}
\end{align}
$$

6.

$$
\begin{align}
\Sigma & = \{ a \} \\
A & = \{ \lambda, a \} \\
B & = \{ \lambda, aa \} \\
 \\
AB  & = \{ aaa \} \\
BA  & = \{ aaa \}
\end{align}
$$

7.

$$
\begin{align}
F(\lambda)  & : \lambda (B C) = (\lambda B) C  \\
  & : BC = (B)C \\
  & : BC = BC
\end{align}
$$

$$
\begin{align}
F(\lambda a) & : \lambda a(BC) = (\lambda aB) C \\
 &: a(BC)
\end{align}
$$

8.

$$
\begin{align}
F(\{ \lambda \} \cdot A) &: u \lambda \quad, u \in A \land v \in \{ \lambda \} \\
&: u \quad, u \in A \\
&: A 
\end{align}
$$


9.

$$
\begin{align}
F(\{ \lambda \} \cdot A) &: u v \quad, u \in A \land v \in \{  \} \\ \\
F(\{ \lambda \} \cdot A) &: u v \quad, u \in A \land v \in F \\
&:  \quad, u \in A \\
&: A 
\end{align}
$$
